Implement chain replication from arbitrary chain

src/Chain_Sync_Mini_Protocol_Implementation.thy
@@ -22,16 +22,27 @@ instance hash :: countable
 
 text \<open> Timing \<close>
 
-type_synonym slot = nat
+type_synonym slot = int
+
+abbreviation
+  genesis_slot :: slot
+where
+  "genesis_slot \<equiv> -1"
 
 text \<open> Blocks \<close>
 
 datatype block =
     GenesisBlock
-  | HeaderBlock "slot \<times> hash option"
+  | HeaderBlock \<open>slot\<close> \<open>hash option\<close>
 
 instance block :: countable
   by countable_datatype
+
+primrec
+  block_slot :: "block \<Rightarrow> slot"
+where
+  "block_slot GenesisBlock = genesis_slot"
+| "block_slot (HeaderBlock slot _) = slot"
 
 text \<open> Chains \<close>
 
@@ -54,11 +65,16 @@ abbreviation (input)
 where
   "genesis_index \<equiv> 0"
 
+text \<open> Points \<close>
+
+type_synonym point = slot (* FIXME: Add hash *)
+
 text \<open> State machines \<close>
 
 (* TODO: Perhaps add a new state StAborted for when the protocol is aborted. *)
 datatype state =
     StIdle
+  | StIntersect
   | StCanAwait
   | StMustReply
   | StDone
@@ -66,8 +82,12 @@ datatype state =
 datatype message =
     MsgDone
   | MsgRequestNext
-  | MsgRollForward block block (* TODO: Find out what the tip is sent for. *)
+  | MsgRollForward \<open>block\<close> \<open>block\<close> (* TODO: Find out what the tip is sent for. *)
+  | MsgRollBackward \<open>point\<close> \<open>block\<close> (* TODO: Find out what the tip is sent for. *)
   | MsgAwaitReply
+  | MsgFindIntersect \<open>point list\<close>
+  | MsgIntersectFound \<open>point\<close> \<open>block\<close> (* TODO: Find out what the tip is sent for. *)
+  | MsgIntersectNotFound \<open>block\<close> (* TODO: Find out what the tip is sent for. *)
 
 instance message :: countable
   by countable_datatype
@@ -78,36 +98,70 @@ type_synonym
   producer_parameters
     = "state \<comment> \<open>current state\<close>
     \<times> chain \<comment> \<open>current chain\<close>
-    \<times> chain_index \<comment> \<open>read pointer\<close>"
+    \<times> chain_index \<comment> \<open>read pointer\<close>
+    \<times> bool \<comment> \<open>whether the next response to @{const MsgRequestNext} should be @{const MsgRollBackward}\<close>"
+
+definition
+  best_intersection_point :: "chain \<Rightarrow> point list \<Rightarrow> point option"
+where
+  [simp]: "best_intersection_point \<C> points = (
+    let
+      intersection_points = List.set points \<inter> List.set (map block_slot \<C>)
+    in
+      if intersection_points = {} then None else Some (Max intersection_points))"
+
+(* NOTE: Assumes that \<exists>index \<in> {0..<length \<C>}. block_slot (\<C> ! index) = slot *)
+definition
+  index_from_slot :: "slot \<Rightarrow> chain \<Rightarrow> chain_index"
+where
+  [simp]: "index_from_slot slot \<C> = hd [index. (block, index) \<leftarrow> zip \<C> [0..<length \<C>], block_slot block = slot]"
 
 definition
   producer
     :: "message channel family
+    \<Rightarrow>  message channel family
     \<Rightarrow>  producer_parameters channel family
     \<Rightarrow>  process family"
 where
-  "producer c pc =
-    pc \<triangleright>\<^sup>\<infinity> (st, \<C>, read_ptr). (
+  "producer CP PC I =
+    I \<triangleright>\<^sup>\<infinity> (st, \<C>, read_ptr, must_rollback). (
       case st of
         StDone \<Rightarrow>
           \<zero> \<comment> \<open>NOTE: Actually the process does not stop here but no longer responds\<close>
       | StMustReply \<Rightarrow>
           \<zero> \<comment> \<open>NOTE: Here the producer waits for updates\<close>
       | _ \<Rightarrow>
-          c \<triangleright> msg. (
+          CP \<triangleright> msg. (
             case (st, msg) of
               (StIdle, MsgDone) \<Rightarrow>
-                pc \<triangleleft> (StDone, \<C>, read_ptr)
+                I \<triangleleft> (StDone, \<C>, read_ptr, must_rollback)
+            | (StIdle, MsgFindIntersect points) \<Rightarrow> (
+                \<comment> \<open>NOTE: StIntersect is only transient, so not used\<close>
+                case best_intersection_point \<C> points of
+                  None \<Rightarrow>
+                    PC \<triangleleft> MsgIntersectNotFound (tip \<C>)
+                    \<parallel>
+                    I \<triangleleft> (StIdle, \<C>, read_ptr, must_rollback)
+                | Some point_intersect \<Rightarrow>
+                    PC \<triangleleft> MsgIntersectFound point_intersect (tip \<C>)
+                    \<parallel>
+                    I \<triangleleft> (StIdle, \<C>, index_from_slot point_intersect \<C>, True))
             | (StIdle, MsgRequestNext) \<Rightarrow>
-                if read_ptr \<le> tip_index \<C>
+                if must_rollback
                   then
-                    c \<triangleleft> MsgRollForward (\<C> ! read_ptr) (tip \<C>)
+                    PC \<triangleleft> MsgRollBackward (block_slot (\<C> ! read_ptr)) (tip \<C>)
                     \<parallel>
-                    pc \<triangleleft> (StCanAwait, \<C>, Suc read_ptr)
+                    I \<triangleleft> (StIdle, \<C>, read_ptr + 1, False)
                   else
-                    c \<triangleleft> MsgAwaitReply
-                    \<parallel>
-                    pc \<triangleleft> (StMustReply, \<C>, read_ptr)
+                    if read_ptr \<le> tip_index \<C>
+                      then
+                        PC \<triangleleft> MsgRollForward (\<C> ! read_ptr) (tip \<C>)
+                        \<parallel>
+                        I \<triangleleft> (StCanAwait, \<C>, Suc read_ptr, must_rollback)
+                      else
+                        PC \<triangleleft> MsgAwaitReply
+                        \<parallel>
+                        I \<triangleleft> (StMustReply, \<C>, read_ptr, must_rollback)
             | (_, _) \<Rightarrow>
                 \<zero> \<comment> \<open>Unexpected message, protocol is aborted\<close>
           )
@@ -120,27 +174,60 @@ type_synonym
     = "state \<comment> \<open>current state\<close>
     \<times> chain \<comment> \<open>current chain\<close>"
 
+(* FIXME: Implement *)
+consts candidate_points :: "chain \<Rightarrow> point list"
+
+definition
+  rollback_to :: "chain \<Rightarrow> point \<Rightarrow> chain"
+where
+  [simp]: "rollback_to \<C> point = takeWhile (\<lambda>block. block_slot block \<le> point) \<C>"
+
 (* FIXME: It doesn't seem to be clear when the consumer should send the MsgDone message. *)
 definition
   consumer
     :: "message channel family
+    \<Rightarrow>  message channel family
     \<Rightarrow>  consumer_parameters channel family
+    \<Rightarrow>  chain option
     \<Rightarrow>  process family"
 where
-  "consumer c cc =
-    cc \<triangleright>\<^sup>\<infinity> (st, \<C>). (
+  "consumer CP PC I o\<C> =
+    (
+    case o\<C> of
+      None \<Rightarrow> \<comment> \<open>No local chain, start from genesis block\<close>
+        I \<triangleleft> (StIdle, [GenesisBlock])
+    | Some \<C> \<Rightarrow> \<comment> \<open>Local chain, find intersection point\<close>
+        \<comment> \<open>NOTE: StIntersect is only transient, so not used\<close>
+        CP \<triangleleft> MsgFindIntersect (candidate_points \<C>)
+        \<parallel>
+        (
+        PC \<triangleright> msg. (
+          case msg of
+            MsgIntersectNotFound tip_point \<Rightarrow>
+              \<zero> \<comment> \<open>FIXME: Abort? Not clear from document\<close>
+          | MsgIntersectFound _ _ \<Rightarrow>
+              \<comment> \<open>TODO: According to the document, the consumer can expect the next update to be
+                  MsgRollBackward, so no need to handle the response here. Confirm.\<close>
+              I \<triangleleft> (StIdle, \<C>)
+          )
+        )
+    )
+    \<parallel>
+    I \<triangleright>\<^sup>\<infinity> (st, \<C>). (
       case st of
         StIdle \<Rightarrow>
-          c \<triangleleft> MsgRequestNext
+          CP \<triangleleft> MsgRequestNext
           \<parallel>
-          cc \<triangleleft> (StCanAwait, \<C>)
+          I \<triangleleft> (StCanAwait, \<C>)
       | StCanAwait \<Rightarrow>
-          c \<triangleright> msg. (
+          PC \<triangleright> msg. (
             case msg of
-              MsgRollForward header pTip \<Rightarrow>
-                cc \<triangleleft> (StIdle, \<C> @ [header])
+              MsgRollForward header tip_point \<Rightarrow>
+                I \<triangleleft> (StIdle, \<C> @ [header])
+            | MsgRollBackward rollback_point tip_point \<Rightarrow>
+                I \<triangleleft> (StIdle, rollback_to \<C> rollback_point)
             | MsgAwaitReply \<Rightarrow>
-                cc \<triangleleft> (StMustReply, \<C>)
+                I \<triangleleft> (StMustReply, \<C>)
             | _ \<Rightarrow>
                 \<zero> \<comment> \<open>Unexpected message, protocol is aborted\<close>
           )
@@ -151,14 +238,16 @@ where
 definition
   protocol
     :: "message channel family
+    \<Rightarrow>  message channel family
     \<Rightarrow>  chain \<comment> \<open>producer's current chain\<close>
+    \<Rightarrow>  chain option \<comment> \<open>consumer's current chain\<close>
     \<Rightarrow>  process family"
 where
-  "protocol c \<C>\<^sub>p =
-    \<nu> pc cc. (
-      producer c pc \<parallel> pc \<triangleleft> (StIdle, \<C>\<^sub>p, Suc genesis_index)
+  "protocol CP PC \<C>\<^sub>p o\<C>\<^sub>c =
+    \<nu> IC IP. (
+      producer CP PC IP \<parallel> IP \<triangleleft> (StIdle, \<C>\<^sub>p, Suc genesis_index, False)
       \<parallel>
-      consumer c cc \<parallel> cc \<triangleleft> (StIdle, [GenesisBlock])
+      consumer CP PC IC o\<C>\<^sub>c
     )"
 
 end
